otbn_model/code/montmul_lemmas.dfy
@@ -1,4 +1,3 @@
-include "../spec/rsa_ops.dfy"
 include "mont_loop_lemmas.dfy"
 
 module montmul_lemmas {
@@ -29,5 +28,49 @@ module montmul_lemmas {
         }
         reveal cong();
         assert montmul_inv(a, x, i, y, key);
+    }
+
+    lemma r_r_inv_cancel_lemma(a: nat, key: pub_key)
+        requires pub_key_inv(key);
+        ensures cong(a * key.R_INV * key.R, a, key.m);
+    {
+        assert cong(key.R_INV * key.R, 1, key.m);
+        cong_mul_lemma_1(key.R_INV * key.R, 1, a, key.m);
+    }
+    
+    lemma r_r_inv_cancel_lemma_2(a: nat, b : nat, key: pub_key)
+        requires pub_key_inv(key);
+        requires cong(a, b * key.R_INV * key.R, key.m);
+        ensures cong(a, b, key.m);
+    {
+        assert cong(b * key.R_INV * key.R, b, key.m) by {
+            r_r_inv_cancel_lemma(b, key);
+        }
+        reveal cong();
+    }
+
+    lemma montmul_inv_lemma_1(a_slice: seq<uint256>,
+        x: seq<uint256>,
+        y: seq<uint256>,
+        key: pub_key)
+    
+        requires montmul_inv(a_slice, x, NUM_WORDS, y, key);
+        ensures cong(to_nat(a_slice), to_nat(x) * to_nat(y) * key.R_INV, key.m);
+    {
+        var m := key.m;
+        var a := to_nat(a_slice);
+        assert x[..NUM_WORDS] == x;
+
+        calc ==> {
+            cong(a * key.R, to_nat(x) * to_nat(y), m);
+                { cong_mul_lemma_1(a * key.R, to_nat(x) * to_nat(y), key.R_INV, m); }
+            cong(a * key.R * key.R_INV, to_nat(x) * to_nat(y) * key.R_INV, m);
+                { reveal cong(); }
+            cong(to_nat(x) * to_nat(y) * key.R_INV, a * key.R * key.R_INV, m);
+                { r_r_inv_cancel_lemma_2(to_nat(x) * to_nat(y) * key.R_INV, a, key); }
+            cong(to_nat(x) * to_nat(y) * key.R_INV, a, m);
+                { reveal cong(); }
+            cong(a, to_nat(x) * to_nat(y) * key.R_INV, m);
+        }
     }
 }
